\section{Backward propagation}
\begin{align}
C &= (a^{(L)} - y)^2. \\
a^{(L)} &= \sigma(z^{(L)}). \\
z^{(L)} &= w^{(L)} a^{(L - 1)} + b^{(L)}.
\end{align}
\begin{align}
\frac{\partial C}{\partial a^{(L)}} &= 2(a^{(L)} - y). \\
\frac{\partial a^{(L)}}{\partial z^{(L)}} &= \sigma^{\prime} (z^{(L)}). \\
\frac{\partial z^{(L)}}{\partial w^{(L)}} &= a^{(L-1)}
\end{align}
\begin{align}
\frac{\partial C}{\partial w^{(L)}} &= 
\frac{\partial z^{(L)}}{\partial w^{(L)}} 
\frac{\partial a^{(L)}}{\partial z^{(L)}}
\frac{\partial C}{\partial a^{(L)}}. \\
&= a^{(L-1)} \sigma^{\prime} (z^{(L)}) 2(a^{(L)} - y). \\
\frac{\partial C}{\partial b^{(L)}} &= 1 \cdot \sigma^{\prime} (z^{(L)}) 2(a^{(L)} - y). \\
\end{align}
In the next-to-last layer,
\begin{align}
\frac{\partial C}{\partial w^{(L-1)}} &= 
\frac{\partial z^{(L-1)}}{\partial w^{(L-1)}}
\frac{\partial a^{(L-1)}}{\partial z^{(L-1)}}
\frac{\partial z^{(L)}}{\partial a^{(L-1)}} 
\frac{\partial a^{(L)}}{\partial z^{(L)}}
\frac{\partial C}{\partial a^{(L)}}. \\
\end{align}

In a general case,
\begin{align}
z_j^{(L)} &= \sum_k w_{jk}^{(L)} a_k^{(L-1)} + b_j^{(L)}
\end{align}

\begin{align}
\nabla C &= \begin{bmatrix}
\frac{\partial C}{\partial w^{(1)}} &
\frac{\partial C}{\partial b^{(1)}} &
\frac{\partial C}{\partial w^{(2)}} &
\frac{\partial C}{\partial b^{(2)}} 
\end{bmatrix}^T
\end{align}
Start with the forward propagation equations
\begin{align}
\mathbf{z}^{(1)} &= W^{(1)} \mathbf{x} +  \mathbf{b}^{(1)}.~(16,) \\
\mathbf{a}^{(1)} &= \sigma^{(1)}(\mathbf{z^{(1)}}).~(16,) \\
\mathbf{z}^{(2)} &= W^{(2)} \mathbf{a^{(1)}} + \mathbf{b}^{(2)}.~(10,) \\
\mathbf{a}^{(2)} &= \sigma^{(2)}(\mathbf{z^{(2)}}).~(10,) \\
C &= |\mathbf{a}^{(2)} - \mathbf{y}|^2 = (a_0^{(2)} - y_0)^2 + (a_1^{(2)} - y_1)^2 + \cdots + (a_9^{(2)} - y_9)^2.
\end{align}
\begin{align}
\begin{bmatrix}
z_0^{(2)} \\
z_1^{(2)} \\
\vdots \\
z_9^{(2)} 
\end{bmatrix}
&= 
\begin{bmatrix}
w_{0,0} & w_{0,1} & \cdots & w_{0,16} \\
w_{1,0} & w_{1,1} & \cdots & w_{1,16} \\
\vdots & \vdots & \cdots & \vdots \\
w_{9,0} & w_{9,1} & \cdots & w_{9,16}
\end{bmatrix}
\begin{bmatrix}
a_0^{(1)} \\
a_1^{(1)} \\
\vdots \\
a_{16}^{(1)} 
\end{bmatrix} 
= 
\begin{bmatrix}
w_{0,0} a_0^{(1)} + w_{0,1} a_1^{(1)} + \cdots + w_{0,16} a_{16}^{(1)} \\
w_{1,0} a_0^{(1)} + w_{1,1} a_1^{(1)} + \cdots + w_{1,16} a_{16}^{(1)} \\
\vdots \\
w_{9,0} a_0^{(1)} + w_{9,1} a_1^{(1)} + \cdots + w_{9,16} a_{16}^{(1)} \\
\end{bmatrix}
\end{align}
Want to find
\begin{align}
\frac{\partial C}{\partial w_{jk}^{(2)}} 
&= 
\frac{\partial z_j^{(2)}}{\partial w_{jk}^{(2)}} 
\frac{\partial a_j^{(2)}}{\partial z_j^{(2)}}
\frac{\partial C}{\partial a_j^{(2)}}. \\
&= a_{k}^{(1)} \sigma^{(2)\prime}(z_j^{(2)}) 2(a_j^{(2)} - y_j) \\
\frac{\partial C}{\partial b_j^{(2)}} 
&= 
\frac{\partial z_j^{(2)}}{\partial b_{j}^{(2)}} 
\frac{\partial a_j^{(2)}}{\partial z_j^{(2)}}
\frac{\partial C}{\partial a_j^{(2)}}. \\
&= \sigma^{(2)\prime}(z_j^{(2)}) 2(a_j^{(2)} - y_j) \\
\frac{\partial C}{\partial w_{jk}^{(1)}} 
&= 
\frac{\partial z_j^{(1)}}{\partial w_{jk}^{(1)}} 
\frac{\partial a_j^{(1)}}{\partial z_{j}^{(1)}} 
\frac{\partial C}{\partial a_{j}^{(1)}} \\
&= a_k^{(0)} \sigma^{(1)\prime} (z_j^{(1)}) \frac{\partial C}{\partial a_{j}^{(1)}} \\
% \frac{\partial z_j^{(1)}}{\partial w_{jk}^{(1)}} 
% \frac{\partial a_k^{(1)}}{\partial z_{j}^{(1)}} 
% \frac{\partial z_m^{(2)}}{\partial a_{k}^{(1)}} 
% \frac{\partial a_m^{(2)}}{\partial z_m^{(2)}}
% \frac{\partial C}{\partial a_m^{(2)}}. \\
% &= x_k^{(1)} \sigma^{(1)\prime}(z_j^{(1)}) w_{m,k} \sigma^{(2)\prime}(z_m^{(2)}) 2(a_m^{(2)} - y_m)
\end{align}
\begin{align}
\frac{\partial C}{\partial a_{j}^{(1)}} 
&= \frac{\partial z_m^{(2)}}{\partial a_{j}^{(1)}} \frac{\partial a_m^{(2)}}{\partial z_{m}^{(2)}} \frac{\partial C}{\partial a_{m}^{(2)}} \\
&= w_{m,j}^{(2)} \sigma^{(2)\prime}(z_m^{(2)}) 2(a_m^{(2)} - y_m)
\end{align}